more

haskell/Optics/Optics/FunList.hs
@@ -9,12 +9,12 @@ module  Optics.FunList
     (   FunList     (..)   
     ,   FunList'    (..)
     ,   FunList_
-    ,   inn
-    ,   out
-    ,   n_to_n
-    ,   sn_to_sn
-    ,   funToFun'
-    ,   fun'ToFun
+    ,   e2fun
+    ,   fun2e
+    ,   nId
+    ,   snId
+    ,   funId
+    ,   fun'Id
     )   where
 
 import Optics.Nat
@@ -22,59 +22,84 @@ import Optics.Vec
 
 data FunList a b t = Done t | More a (FunList a b (b -> t))
 
-out :: FunList a b t -> Either t (a, FunList a b (b -> t))
-out (Done t)    = Left t
-out (More x l)  = Right (x,l) 
+fun2e :: FunList a b t -> Either t (a, FunList a b (b -> t))
+fun2e (Done t)    = Left t
+fun2e (More x l)  = Right (x,l) 
 
-inn :: Either t (a, FunList a b (b -> t)) -> FunList a b t
-inn (Left t)        = Done t
-inn (Right (x,l))   = More x l
+e2fun :: Either t (a, FunList a b (b -> t)) -> FunList a b t
+e2fun (Left t)        = Done t
+e2fun (Right (x,l))   = More x l
 
--- (inn . out) (Done t)   = inn (Left t) = Done t
--- (inn . out) (More x l) = inn (Right (x,l)) = More x l
+-- (e2fun . fun2e) (Done t)   = e2fun (Left t) = Done t
+-- (e2fun . fun2e) (More x l) = e2fun (Right (x,l)) = More x l
 
--- (out . inn) (Left t) = out (Done t) = Left t
--- (out . inn) (Right (x,l)) = out (More x l) = Right (x,l)
+-- (fun2e . e2fun) (Left t) = fun2e (Done t) = Left t
+-- (fun2e . e2fun) (Right (x,l)) = fun2e (More x l) = Right (x,l)
 
 
 type FunList_ (n :: Nat) a b t = (Vec n a, Vec n b -> t)
 
 -- FunList_ ('S n) a b t and (a, FunList_ n a b (b -> t)) are isomorphic
 
-n_to_sn :: (a, FunList_ n a b (b -> t)) -> FunList_ ('S n) a b t
-n_to_sn (a, (vec, f)) = (Cons a vec, g) where
+n2sn :: (a, FunList_ n a b (b -> t)) -> FunList_ ('S n) a b t
+n2sn (a, (vec, f)) = (Cons a vec, g) where
     g (Cons b vec') = f vec' b
 
-sn_to_n :: FunList_ ('S n) a b t -> (a, FunList_ n a b (b -> t))
-sn_to_n (Cons a vec, f) = (a, (vec, g)) where 
+sn2n :: FunList_ ('S n) a b t -> (a, FunList_ n a b (b -> t))
+sn2n (Cons a vec, f) = (a, (vec, g)) where 
     g vec' b = f (Cons b vec')
 
-n_to_n :: (a, FunList_ n a b (b -> t)) -> (a, FunList_ n a b (b -> t))
-n_to_n = sn_to_n . n_to_sn
+nId :: (a, FunList_ n a b (b -> t)) -> (a, FunList_ n a b (b -> t))
+nId = sn2n . n2sn
 
-sn_to_sn :: FunList_ ('S n) a b t -> FunList_ ('S n) a b t 
-sn_to_sn = n_to_sn . sn_to_n
+snId :: FunList_ ('S n) a b t -> FunList_ ('S n) a b t 
+snId = n2sn . sn2n
 
 data FunList' a b t where
      FunList' :: forall (n :: Nat) a b t . FunList_ n a b t -> FunList' a b t
 
 
-funToFun' :: FunList a b t -> FunList' a b t
-funToFun' (Done t) = FunList' (Nil, \_ -> t)
-funToFun' (More a fun) = case funToFun' fun of
-   (FunList' fun_n) -> FunList' $ n_to_sn (a , fun_n)
+fun2fun' :: FunList a b t -> FunList' a b t
+fun2fun' (Done t) = FunList' (Nil, \_ -> t)
+fun2fun' (More a fun) = case fun2fun' fun of
+   (FunList' (vec,f)) -> FunList' $ n2sn (a , (vec,f))
 
-fun'ToFun :: FunList' a b t -> FunList a b t
-fun'ToFun (FunList' (Nil, f)) = Done (f Nil)
-fun'ToFun (FunList' (Cons a vec, f)) = case sn_to_n (Cons a vec, f) of
-    (a', (vec', g)) -> More a' (fun'ToFun (FunList' (vec', g))) 
+fun'2fun :: FunList' a b t -> FunList a b t
+fun'2fun (FunList' (Nil, f)) = Done (f Nil)
+fun'2fun (FunList' (Cons a vec, f)) = case sn2n (Cons a vec, f) of
+    (a', (vec', g)) -> More a' (fun'2fun (FunList' (vec', g))) 
+
+funId :: FunList a b t -> FunList a b t 
+funId = fun'2fun . fun2fun'
+
+fun'Id :: FunList' a b t -> FunList' a b t 
+fun'Id = fun2fun' . fun'2fun
 
 -- pseudo haskell proof
 
--- n_to_n (a, (vec, f))
--- = (sn_to_n . n_to_sn) (a, (vec f))
--- = sn_to_n (n_to_sn (a, (vec f)))
--- = sn_to_n (Cons a vec, g)            [g (Cons b vec') = f vec' b]
+-- funId (Done t) 
+-- = (fun'2fun . fun2fun') (Done t)
+-- = fun'2fun (fun2fun' (Done t))
+-- = fun'2fun (FunList' (Nil, \_ -> t))
+-- = Done ((\_ -> t) Nil)
+-- = Done t
+--
+-- funId (More a fun)
+-- = (fun'2fun . fun2fun') (More a fun)
+-- = fun'2fun (fun2fun' (More a fun))
+-- = fun'2fun (FunList' (n2sn (a, (vec, f)))) [FunList' (vec,f) = fun2fun' fun]
+-- = fun'2fun (FunList' (Cons a vec, g))      [g (Cons b vec') = f vec' b     ] 
+-- = More a' (fun'2fun (FunList' (vec',g')))  
+-- where
+-- (a', (vec',g')) 
+-- = sn2n (Cons a vec, g)
+-- = (a, (vec, g'))         [g' vec' b = g (Cons b vec')]    
+--
+
+-- nId (a, (vec, f))
+-- = (sn2n . n2sn) (a, (vec f))
+-- = sn2n (n2sn (a, (vec f)))
+-- = sn2n (Cons a vec, g)               [g (Cons b vec') = f vec' b]
 -- = (a, (vec, g'))                     [g' vec' b = g (Cons b vec')]
 -- = (a, (vec, f))                      [need to show g' = f ]
 -- proof of g' = f
@@ -85,10 +110,10 @@ fun'ToFun (FunList' (Cons a vec, f)) = case sn_to_n (Cons a vec, f) of
 -- = g (Cons b vec')
 -- = f vec' b
 
--- sn_to_sn (Cons a vec, f)
--- = (n_to_sn . sn_to_n) (Cons a vec, f)
--- = n_to_sn (sn_to_n (Cons a vec, f))
--- = n_to_sn (a, (vec , g))     [g vec' b = f (Cons b vec')]
+-- snId (Cons a vec, f)
+-- = (n2sn . sn2n) (Cons a vec, f)
+-- = n2sn (sn2n (Cons a vec, f))
+-- = n2sn (a, (vec , g))        [g vec' b = f (Cons b vec')]
 -- = (Cons a vec, g')           [g' (Cons b vec') = g vec' b]
 -- = (Cons a vec, f)            [since g' = f :: Vec ('S n) b -> t]
 
