haskell/Optics/Optics/Test/FunList.hs
@@ -1,6 +1,11 @@
 module  Optics.Test.FunList
     (   specFunList
     ,   FunList
+    , t1 
+    , t2
+    , t3
+    , t4
+    , t5
     )   where
 
 import Test.Hspec
@@ -10,3 +15,21 @@ specFunList :: Spec
 specFunList = describe "Testing FunList..." $ do
     it "Checked module compiled" $
         True `shouldBe` True
+
+
+type T t = FunList Int Bool t
+
+t1 :: T String
+t1 = Done "hello"
+
+t2 :: T (Bool -> String)
+t2 = Done show
+
+t3 :: T String
+t3 = More 0 t2
+
+t4 :: T (Bool -> Bool -> String)
+t4 = Done (\x y -> show x ++ ":" ++ show y)
+
+t5 :: T String
+t5 = More 1 (More 0 t4)
