coq/ref/Vec.v
@@ -1,0 +1,23 @@
+Inductive Vec : nat -> Type -> Type :=
+| Nil   : forall (a:Type), Vec 0 a
+| Cons  : forall (n:nat) (a:Type), a -> Vec n a -> Vec (S n) a
+.
+
+Check Vec.
+
+Arguments Nil {a}.
+
+Arguments Cons {n} {a}.
+
+
+Definition cast1 (a:Type) (m:nat) (xs:Vec m a) : Vec (0 + m) a := xs.
+
+Arguments cast1 {a} {m}.
+
+
+Fixpoint append (a:Type) (n m:nat) (xs:Vec n a) (ys:Vec m a) : Vec (n + m) a :=
+    match xs in Vec n' a' return Vec (n' + m) a' with
+    | @Nil _        => cast1 ys
+    | Cons x xs'    => Cons x (append _ _ _ xs' ys)
+    end. 
+
