coq/set/Semantics/Empty.v
@@ -1,0 +1,16 @@
+Require Import Core.LEM.
+Require Import Core.Set.
+Require Import Core.Elem.
+Require Import Core.Syntax.
+Require Import Core.Semantics.
+Require Import Core.Environment.
+
+(* Theorem 'emptySet' expressed in set theory abstract syntax.                  *)
+Definition emptySetF : Formula := Exi 0 (All 1 (Not (Elem 1 0))).
+
+(* Evaluating emptySetF in any environment 'yields' the theorem emptySet.       *)
+Lemma evalEmptySetF : LEM -> forall (e:Env),
+    eval e emptySetF <-> exists (x:set), forall (z:set), ~ (z :: x).
+Proof.
+    intros L e. apply evalExi. assumption.
+Qed.
