coq/set/Semantics/Equal.v
@@ -1,0 +1,104 @@
+Require Import Core.LEM.
+Require Import Core.Set.
+Require Import Core.Incl.
+Require Import Core.Elem.
+Require Import Core.Equal.
+Require Import Core.Syntax.
+Require Import Core.Semantics.
+Require Import Core.Environment.
+
+(* Lemma 'equalRefl' expressed in set theory abstract syntax.                   *)
+Definition equalReflF (n:nat) : Formula := All n (Equ n n).
+
+(* Evaluating equalReflF in any environment 'yields' the lemma equalRefl.       *)
+Lemma evalEqualReflF : LEM -> forall (e:Env) (n:nat), 
+    eval e (equalReflF n) <-> forall (x:set), x == x.
+Proof.
+    intros L e n. unfold equalReflF. rewrite evalAll. split; intros H x.
+    - remember (H x) as H' eqn:E. clear E. clear H.
+      rewrite evalEqu in H'. rewrite bindSame in H'. 
+        + assumption.
+        + assumption.
+    - rewrite evalEqu, bindSame. apply H.
+        + assumption.
+Qed.
+
+(* Lemma 'equalSym' expressed in set theory abstract syntax.                    *)
+(* This formulation is correct when variables n and m are distinct.             *)
+Definition equalSymF (n m:nat):Formula:= All n (All m (Imp (Equ n m) (Equ m n))).
+
+(* Evaluating equalSymF in any environment 'yields' the lemma equalSym.         *)
+Lemma evalEqualSymF : LEM -> forall (e:Env) (n m:nat), 
+    m <> n -> 
+    eval e (equalSymF n m) 
+        <->     
+    forall (x y:set), x == y -> y == x.
+Proof.
+    intros L e n m Hmn. unfold equalSymF. rewrite evalAll. split; intros H x.
+    - intros y.
+      remember (H  x) as H' eqn:E. clear E. clear H. rewrite evalAll in H'. 
+      remember (H' y) as H  eqn:E. clear E. clear H'.
+      rewrite evalImp in H. rewrite evalEqu in H. rewrite evalEqu in H.
+      remember (bind e n x) as e1 eqn:E1.
+      rewrite bindSame in H. rewrite bindDiff in H. rewrite E1 in H.
+      rewrite bindSame in H.
+        + assumption.
+        + assumption.
+        + assumption.
+        + assumption.
+    - rewrite evalAll. intros y. remember (bind e n x) as e1 eqn:E1.
+      rewrite evalImp, evalEqu, evalEqu, bindSame, bindDiff, E1, bindSame.
+        + apply H.
+        + assumption.
+        + assumption.
+        + assumption.
+Qed.
+
+(* Lemma 'equalTrans' expressed in set theory abstract syntax.                  *)
+(* This formulation is correct when variables n m p are distinct.               *)
+Definition equalTransF (n m p:nat) : Formula := 
+    All n (All m (All p (Imp (Equ n m) (Imp (Equ m p) (Equ n p))))).
+
+(* Evaluating equalTransF in any environment 'yields' the lemma equalTrans.     *)
+Lemma evalEqualTransF : LEM -> forall (e:Env) (n m p:nat), 
+    m <> n -> 
+    p <> m -> 
+    p <> n ->
+    eval e (equalTransF n m p)
+        <-> 
+    forall (x y z:set), x == y -> y == z -> x == z.
+Proof.
+    intros L e n m p Hmn Hpm Hpn. unfold equalTransF. rewrite evalAll. split; 
+    intros H x.
+    - intros y z.
+      remember (H x) as H' eqn:E. clear E. clear H.  rewrite evalAll in H'.
+      remember (H' y) as H eqn:E. clear E. clear H'. rewrite evalAll in H.
+      remember (H z) as H' eqn:E. clear E. clear H.
+      rewrite evalImp in H'. rewrite evalImp in H'.
+      rewrite evalEqu in H'. rewrite evalEqu in H'. rewrite evalEqu in H'.
+      remember (bind e n x)  as e1 eqn:E1.
+      remember (bind e1 m y) as e2 eqn:E2.
+      rewrite bindSame in H'. rewrite bindDiff in H'. rewrite bindDiff in H'.
+      rewrite E2 in H'. rewrite bindSame in H'. rewrite bindDiff in H'.
+      rewrite E1 in H'. rewrite bindSame in H'.
+        + assumption.
+        + assumption.
+        + assumption.
+        + assumption.
+        + assumption.
+        + assumption.
+        + assumption.
+    - rewrite evalAll. intros y. rewrite evalAll. intros z.
+      remember (bind e n x)  as e1 eqn:E1.
+      remember (bind e1 m y) as e2 eqn:E2.
+      rewrite evalImp, evalImp, evalEqu, evalEqu, evalEqu.
+      rewrite bindSame, bindDiff, bindDiff, E2, bindSame, bindDiff, E1.
+      rewrite bindSame.
+        + apply H.
+        + assumption.
+        + assumption.
+        + assumption.
+        + assumption.
+        + assumption.
+        + assumption.
+Qed.
