coq/set/Semantics/Incl.v
@@ -1,0 +1,35 @@
+Require Import Core.LEM.
+Require Import Core.Set.
+Require Import Core.Incl.
+Require Import Core.Syntax.
+Require Import Core.Semantics.
+Require Import Core.Environment.
+
+(* Lemma 'inclRefl' expressed in set theory abstract syntax.                    *)
+Definition inclReflF (n:nat) : Formula := All n (Sub n n).
+
+(* The intent is to provide some validation to our semantics by going through   *)
+(* several key set theoretic results and proving the equivalence between the    *)
+(* evaluated abstract syntax and the corresponding Coq statement. However, the  *)
+(* value of such exercise is limited as a Coq equivalence 'A <-> B' can always  *)
+(* be proved whenever A and B are themselves provable. So 'A <-> B' does not in *)
+(* itself prove that the propositions A and B are the 'same'. For our defense,  *)
+(* we are proving the equivalence 'A <-> B' without using any result which      *)
+(* asserts A or B. In particular, we make no use of the lemma 'inclRefl'.       *)
+(* With this caveat in mind, we assert that evaluating inclReflF in any         *)
+(* environment (and for any choice of variable name 'n') yields a proposition   *)
+(* which is equivalent to the lemma inclRefl.                                   *)
+Lemma evalInclReflF : LEM -> forall (e:Env) (n:nat),
+    eval e (inclReflF n) <-> forall (x:set), x <== x.
+Proof.
+    intros L e n. unfold inclReflF. rewrite evalAll. split; intros H x.
+    - remember (H x) as H' eqn:E. clear E. 
+      rewrite evalSub in H'. 
+        + rewrite bindSame in H'. assumption.
+        + assumption.
+    - rewrite evalSub.
+        + rewrite bindSame. apply H.
+        + assumption.
+Qed.        
+
+
