coq/set/Semantics/Trans.v
@@ -1,0 +1,58 @@
+Require Import Core.LEM.
+Require Import Core.Set.
+Require Import Core.Incl.
+Require Import Core.Syntax.
+Require Import Core.Semantics.
+Require Import Core.Environment.
+
+(* Theorem 'inclTrans' expressed in set theory abstract syntax.                 *)
+(* This formulation is correct when variables n m p are distinct.               *)
+Definition inclTransF (n m p:nat) : Formula := 
+    All n (All m (All p (Imp (Sub n m) (Imp (Sub m p) (Sub n p))))).
+
+(* Evaluating inclTransF in any environment 'yields' the theorem inclTrans.     *)
+Lemma evalTransReflF : LEM -> forall (e:Env) (n m p:nat), 
+    m <> n -> 
+    p <> m -> 
+    p <> n ->
+    eval e (inclTransF n m p) 
+        <-> 
+    forall (x y z:set), x <== y -> y <== z -> x <== z. 
+Proof.
+    intros L e n m p Hmn Hpm Hpn. unfold inclTransF. rewrite evalAll. split.
+    - intros H x y z. 
+      remember (H x) as H' eqn:E. clear E. clear H.
+      rewrite evalAll in H'.
+      remember (H' y) as H eqn:E. clear E. clear H'.
+      rewrite evalAll in H.
+      remember (H z) as H' eqn:E. clear E. clear H.
+      rewrite evalImp in H'. rewrite evalImp in H'.
+      rewrite evalSub in H'. rewrite evalSub in H'. rewrite evalSub in H'.
+      remember (bind e n x)  as e1 eqn:E1.
+      remember (bind e1 m y) as e2 eqn:E2.
+      rewrite bindDiff in H'. rewrite bindDiff in H'. rewrite bindSame in H'.
+      rewrite E2 in H'. rewrite bindDiff in H'. rewrite bindSame in H'.
+      rewrite E1 in H'. rewrite bindSame in H'.
+        + assumption.
+        + assumption.
+        + assumption.
+        + assumption.
+        + assumption.
+        + assumption.
+        + assumption.
+    - intros H x. rewrite evalAll. intros y. rewrite evalAll. intros z.
+      remember (bind e n x)  as e1 eqn:E1.
+      remember (bind e1 m y) as e2 eqn:E2.
+      remember (bind e2 p z) as e3 eqn:E3.
+      rewrite evalImp, evalImp, evalSub, evalSub, evalSub, E3. 
+      rewrite bindSame, bindDiff, bindDiff, E2.
+      rewrite bindSame, bindDiff, E1, bindSame.
+        + apply H.
+        + assumption.
+        + assumption.
+        + assumption.
+        + assumption.
+        + assumption.
+        + assumption.
+Qed.
+
