agda/plfa/relations.agda
@@ -279,6 +279,40 @@ data odd where
     → odd (suc n)
 
 
+e+e≡e : ∀ {m n : ℕ}
+  →  even m
+  →  even n
+    ----------
+  →  even (m + n)
+
+
+o+e≡o : ∀ {m n : ℕ}
+  →  odd m
+  →  even n
+    ----------
+  →  odd (m + n)
+
+e+e≡e zero en = en
+e+e≡e (suc om) en = suc (o+e≡o om en)
+
+o+e≡o (suc em) en = suc (e+e≡e em en)
+
+
+e+o≡o : ∀ {m n : ℕ}
+  →  even m
+  →  odd n
+    ----------
+  →  odd (m + n)
+
+e+o≡o {m} {n} em on rewrite +-comm m n = o+e≡o on em
+
+o+o≡e : ∀ {m n : ℕ}
+  →  odd m
+  →  odd n
+    ----------
+  →  even (m + n)
+
+o+o≡e (suc em) on = suc (e+o≡o em on)
 
 
 
